solvers/54.lean
@@ -4,4 +4,4 @@ open ProjectEulerSolutions.P54
 
 def main : IO Unit := do
   let text ← IO.FS.readFile "0054_poker.txt"
-  IO.println (solve (parseLines text))
+  IO.println (solveLines (parseLines text))
