solvers/60.lean
@@ -3,4 +3,4 @@ import ProjectEulerSolutions.P60
 open ProjectEulerSolutions.P60
 
 def main : IO Unit := do
-  IO.println (solve 10000)
+  IO.println (solve 5)
